thys/Transition_Systems_and_Automata/Automata/BA.thy
@@ -9,39 +9,59 @@ imports
 begin
 
   record ('label, 'state) ba =
-    succ :: "'label \<Rightarrow> 'state \<Rightarrow> 'state set"
+    alphabet :: "'label set"
     initial :: "'state set"
+    succ :: "'label \<Rightarrow> 'state \<Rightarrow> 'state set"
     accepting :: "'state \<Rightarrow> bool"
 
   global_interpretation ba: transition_system_initial
-    "\<lambda> (a, q) p. q" "\<lambda> (a, q) p. q \<in> succ A a p" "\<lambda> p. p \<in> initial A"
+    "\<lambda> a p. snd a" "\<lambda> a p. fst a \<in> alphabet A \<and> snd a \<in> succ A (fst a) p" "\<lambda> p. p \<in> initial A"
     for A
-    defines path = ba.path and run = ba.run and reachable = ba.reachable and nodes = ba.nodes
+    defines path = ba.path and run = ba.run and reachable = ba.reachable and nodes = ba.nodes and
+      enableds = ba.enableds and paths = ba.paths and runs = ba.runs
     by this
 
   abbreviation "target \<equiv> ba.target"
   abbreviation "states \<equiv> ba.states"
   abbreviation "trace \<equiv> ba.trace"
 
+  lemma states_alt_def: "states r p = map snd r" by (induct r arbitrary: p) (auto)
+  lemma trace_alt_def: "trace r p = smap snd r" by (coinduction arbitrary: r p) (auto)
+
   abbreviation successors :: "('label, 'state, 'more) ba_scheme \<Rightarrow> 'state \<Rightarrow> 'state set" where
     "successors \<equiv> ba.successors TYPE('label) TYPE('more)"
 
-  lemma states_alt_def: "states r p = map snd r" by (induct r arbitrary: p) (auto)
-  lemma trace_alt_def: "trace r p = smap snd r" by (coinduction arbitrary: r p) (auto split: prod.splits)
+  lemma successors_alt_def: "successors A p = (\<Union> a \<in> alphabet A. succ A a p)" by auto
 
   abbreviation "pred A a q \<equiv> {p. q \<in> succ A a p}"
 
-  definition language :: "('label, 'state) ba \<Rightarrow> 'label stream set" where
-    "language A \<equiv> {smap fst r |r p. run A r p \<and> p \<in> initial A \<and> infs (accepting A) (trace r p)}"
+  lemma reachable_succ[intro]:
+    assumes "a \<in> alphabet A" "q \<in> reachable A p" "r \<in> succ A a q"
+    shows "r \<in> reachable A p"
+    using ba.reachable.execute assms by force
+  lemma nodes_succ[intro]:
+    assumes "a \<in> alphabet A" "p \<in> nodes A" "q \<in> succ A a p"
+    shows "q \<in> nodes A"
+    using ba.nodes.execute assms by force
+
+  definition language :: "('label, 'state, 'more) ba_scheme \<Rightarrow> 'label stream set" where
+    "language A \<equiv> {w |w r p. p \<in> initial A \<and> run A (w ||| r) p \<and> infs (accepting A) (trace (w ||| r) p)}"
 
   lemma language[intro]:
-    assumes "run A (w ||| r) p" "p \<in> initial A" "infs (accepting A) (trace (w ||| r) p)"
+    assumes "p \<in> initial A" "run A (w ||| r) p" "infs (accepting A) (trace (w ||| r) p)"
     shows "w \<in> language A"
-    using assms unfolding language_def by (auto iff: split_szip_ex)
+    using assms unfolding language_def by auto
   lemma language_elim[elim]:
     assumes "w \<in> language A"
     obtains r p
-    where "run A (w ||| r) p" "p \<in> initial A" "infs (accepting A) (trace (w ||| r) p)"
-    using assms unfolding language_def by (auto iff: split_szip_ex)
+    where "p \<in> initial A" "run A (w ||| r) p" "infs (accepting A) (trace (w ||| r) p)"
+    using assms unfolding language_def by auto
+
+  lemma run_alphabet:
+    assumes "run A (w ||| r) p"
+    shows "w \<in> streams (alphabet A)"
+    using assms by (coinduction arbitrary: w r p) (metis ba.run.cases stream.map szip_smap szip_smap_fst)
+  lemma language_alphabet: "language A \<subseteq> streams (alphabet A)"
+    unfolding language_def by (auto dest: run_alphabet)
 
 end
