thys/Buchi_Complementation/Complementation_Final.thy
@@ -1,0 +1,93 @@
+section {* Complementation to Explicit Büchi Automaton *}
+
+theory Complementation_Final
+imports
+  "Complementation_Implement"
+  "Transition_Systems_and_Automata.BA_Translate"
+begin
+
+  lemma complement_3_finite[simp]:
+    assumes "finite (nodes A)"
+    shows "finite (nodes (complement_3 A))"
+  proof -
+    have "(nodes (complement_3 A), nodes (complement_2 A)) \<in> \<langle>Id\<rangle> set_rel"
+      using complement_3_refine by parametricity auto
+    also have "(nodes (complement_2 A), nodes (complement_1 A)) \<in> \<langle>Id\<rangle> set_rel"
+      using complement_2_refine by parametricity auto
+    also have "(nodes (complement_1 A), nodes (complement A)) \<in> \<langle>cs_rel\<rangle> set_rel"
+      using complement_1_refine by parametricity auto
+    finally have 1: "(nodes (complement_3 A), nodes (complement A)) \<in> \<langle>cs_rel\<rangle> set_rel" by simp
+    have "finite (nodes (complement A))" using complement_finite assms(1) by this
+    then show "finite (nodes (complement_3 A))"
+      using finite_set_rel_transfer_back[OF 1 cs_rel_inv_single_valued] by simp
+  qed
+  lemma complement_3_language[simp]:
+    assumes "finite (nodes A)"
+    shows "language (complement_3 A) = streams (alphabet A) - language A"
+  proof -
+    have "(language (complement_3 A), language (complement_2 A)) \<in> \<langle>\<langle>Id\<rangle> stream_rel\<rangle> set_rel"
+      using complement_3_refine by parametricity auto
+    also have "(language (complement_2 A), language (complement_1 A)) \<in> \<langle>\<langle>Id\<rangle> stream_rel\<rangle> set_rel"
+      using complement_2_refine by parametricity auto
+    also have "(language (complement_1 A), language (complement A)) \<in> \<langle>\<langle>Id\<rangle> stream_rel\<rangle> set_rel"
+      using complement_1_refine by parametricity auto
+    also have "language (complement A) = streams (alphabet A) - language A"
+      using complement_language assms(1) by this
+    finally show "language (complement_3 A) = streams (alphabet A) - language A" by simp
+  qed
+
+  term list_map_rel
+  definition state_hash :: "nat \<Rightarrow> (nat \<times> item) list \<Rightarrow> nat" where
+    "state_hash n p \<equiv> undefined"
+
+  (* TODO: bot is a terrible hash function *)
+  lemma [autoref_ga_rules]: "is_bounded_hashcode
+    state_rel
+    (gen_equals (Gen_Map.gen_ball (foldli \<circ> list_map_to_list)) (list_map_lookup HOL.eq) (prod_eq HOL.eq HOL.eq))
+    bot"
+    apply rule
+    subgoal by autoref
+    subgoal unfolding bot_fun_def bot_nat_def by simp
+    subgoal unfolding bot_fun_def bot_nat_def by simp
+    done
+
+  schematic_goal complement_impl:
+    assumes [simp]: "finite (nodes A)"
+    assumes [autoref_rules]: "(Ai, A) \<in> \<langle>Id, nat_rel, unit_rel\<rangle> bai_ba_rel"
+    shows "(?f :: ?'c, to_baei (complement_3 A)) \<in> ?R"
+    by autoref
+  concrete_definition complement_impl uses complement_impl[unfolded autoref_tag_defs]
+
+  theorem
+    assumes "finite (nodes A)"
+    assumes "(Ai, A) \<in> \<langle>Id, nat_rel, unit_rel\<rangle> bai_ba_rel"
+    shows "language (bae_ba (bae (complement_impl Ai))) = streams (alphabet A) - language A"
+  proof -
+    have "(language ((bae_ba \<circ> bae) (complement_impl Ai)), language (id (complement_3 A))) \<in>
+      \<langle>\<langle>Id_on (alphabet (complement_3 A))\<rangle> stream_rel\<rangle> set_rel"
+      using complement_impl.refine[OF assms, unfolded to_baei_def id_apply] by parametricity
+    also have "language (id (complement_3 A)) = streams (alphabet A) - language A"
+      using assms(1) by simp
+    finally show ?thesis by simp
+  qed
+
+  definition s where
+    "s a p \<equiv> if p = 0
+      then (if a = ''a'' then [0, 1] else [1])
+      else (if a = ''a'' then [1] else [])"
+  definition Ai where
+    "Ai \<equiv> \<lparr> alphabeti = [''a'', ''b''], initiali = [0], succi = s, acceptingi = \<lambda> p. False \<rparr>"
+
+  (* TODO: look through code
+    - equality on maps needs a lot of lookups, make sure those are fast,
+    - make sure we don't use slow generic algorithms when fast specializations are possible *)
+  (* TODO: the reachability analysis should only be done once *)
+  export_code complement_impl in SML module_name Complementation
+
+  (* TODO: is it supposed to be this many states/transitions?
+    make sure that we generate only one representative per equivalence class (maybe prove?)
+    maybe we can also do some crude optimizations *)
+  value "length (transei (complement_impl Ai))"
+  value "length (remdups (map fst (transei (complement_impl Ai))))"
+
+end
