thys/Transition_Systems_and_Automata/Transition_Systems/Transition_System_Refine.thy
@@ -3,6 +3,7 @@ section {* Refinement for Transition Systems *}
 theory Transition_System_Refine
 imports
   "Transition_System"
+  "Transition_System_Extra"
   "../Basic/Refine"
 begin
 
@@ -38,6 +39,89 @@ begin
       show "A.run r p" if "(r, s) \<in> \<langle>T\<rangle> stream_rel" "(p, q) \<in> S" "B.run s q" for r s p q
         using 1[param_fo] that by (coinduction arbitrary: r s p q) (blast elim: stream_rel_cases)
     qed
+  qed
+
+  lemma paths_param[param]:
+    assumes [param]: "(exa, exb) \<in> T \<rightarrow> S \<rightarrow> S"
+    assumes "(transition_system.enableds ena, transition_system.enableds enb) \<in> S \<rightarrow> \<langle>T\<rangle> set_rel"
+    shows "(transition_system.paths exa ena, transition_system.paths exb enb) \<in> S \<rightarrow> \<langle>\<langle>T\<rangle> list_rel\<rangle> set_rel"
+  proof -
+    note assms = assms[param_fo, unfolded transition_system.enableds_def]
+    interpret A: transition_system exa ena by this
+    interpret B: transition_system exb enb by this
+    have 1: "\<exists> s. (r, s) \<in> \<langle>T\<rangle> list_rel \<and> B.path s q" if "(p, q) \<in> S" "A.path r p" for p q r
+    using that(2, 1)
+    proof (induct arbitrary: q)
+      case (nil p)
+      show ?case by auto
+    next
+      case (cons a p r)
+      obtain b where 1: "(a, b) \<in> T" "enb b q" using assms(2) cons(1, 4) by (blast elim: set_relE1)
+      have 2: "(exa a p, exb b q) \<in> S" using cons(4) 1(1) by parametricity
+      obtain s where 3: "(r, s) \<in> \<langle>T\<rangle> list_rel" "B.path s (exb b q)" using cons(3) 2 by auto
+      show ?case using 1 3 by force
+    qed
+    have 2: "\<exists> r. (r, s) \<in> \<langle>T\<rangle> list_rel \<and> A.path r p" if "(p, q) \<in> S" "B.path s q" for p q s
+    using that(2, 1)
+    proof (induct arbitrary: p)
+      case (nil q)
+      show ?case by auto
+    next
+      case (cons b q s)
+      obtain a where 1: "(a, b) \<in> T" "ena a p" using assms(2) cons(1, 4) by (blast elim: set_relE2)
+      have 2: "(exa a p, exb b q) \<in> S" using cons(4) 1(1) by parametricity
+      obtain r where 3: "(r, s) \<in> \<langle>T\<rangle> list_rel" "A.path r (exa a p)" using cons(3) 2 by auto
+      show ?case using 1 3 by force
+    qed
+    show ?thesis unfolding transition_system.paths_def set_rel_def using 1 2 by blast
+  qed
+  lemma runs_param[param]:
+    assumes "(exa, exb) \<in> T \<rightarrow> S \<rightarrow> S"
+    assumes "(transition_system.enableds ena, transition_system.enableds enb) \<in> S \<rightarrow> \<langle>T\<rangle> set_rel"
+    shows "(transition_system.runs exa ena, transition_system.runs exb enb) \<in> S \<rightarrow> \<langle>\<langle>T\<rangle> stream_rel\<rangle> set_rel"
+  proof -
+    note assms = assms[param_fo, unfolded transition_system.enableds_def]
+    interpret A: transition_system exa ena by this
+    interpret B: transition_system exb enb by this
+    have 1: "\<exists> s. (r, s) \<in> \<langle>T\<rangle> stream_rel \<and> B.run s q" if "(p, q) \<in> S" "A.run r p" for p q r
+    proof -
+      define P where "P \<equiv> \<lambda> (p, q, r). (p, q) \<in> S \<and> A.run r p"
+      define Q where "Q \<equiv> \<lambda> (p :: 'b, q, r) a. (shd r, a) \<in> T \<and> enb a q"
+      have 1: "P (p, q, r)" using that unfolding P_def by auto
+      have "\<exists> a. Q x a" if "P x" for x
+        using assms(2) that unfolding P_def Q_def by (force elim: set_relE1 A.run.cases)
+      then obtain f where 2: "\<And> x. P x \<Longrightarrow> Q x (f x)" by metis
+      define g where "g \<equiv> \<lambda> (p, q, r). (exa (shd r) p, exb (f (p, q, r)) q, stl r)"
+      have 3: "P (g x)" if "P x" for x
+        using assms(1) 2 that unfolding P_def Q_def g_def by (auto elim: A.run.cases)
+      show ?thesis
+      proof (intro exI conjI)
+        show "(r, smap f (siterate g (p, q, r))) \<in> \<langle>T\<rangle> stream_rel"
+          using 1 2 3 unfolding Q_def g_def by (coinduction arbitrary: p q r) (fastforce)
+        show "B.run (smap f (siterate g (p, q, r))) q"
+          using 1 2 3 unfolding Q_def g_def by (coinduction arbitrary: p q r) (fastforce)
+      qed
+    qed
+    have 2: "\<exists> r. (r, s) \<in> \<langle>T\<rangle> stream_rel \<and> A.run r p" if "(p, q) \<in> S" "B.run s q" for p q s
+    proof -
+      define P where "P \<equiv> \<lambda> (p, q, s). (p, q) \<in> S \<and> B.run s q"
+      define Q where "Q \<equiv> \<lambda> (p, q :: 'd, s) b. (b, shd s) \<in> T \<and> ena b p"
+      have 1: "P (p, q, s)" using that unfolding P_def by auto
+      have "\<exists> a. Q x a" if "P x" for x
+        using assms(2) that unfolding P_def Q_def by (force elim: set_relE2 B.run.cases)
+      then obtain f where 2: "\<And> x. P x \<Longrightarrow> Q x (f x)" by metis
+      define g where "g \<equiv> \<lambda> (p, q, s). (exa (f (p, q, s)) p, exb (shd s) q, stl s)"
+      have 3: "P (g x)" if "P x" for x
+        using assms(1) 2 that unfolding P_def Q_def g_def by (auto elim: B.run.cases)
+      show ?thesis
+      proof (intro exI conjI)
+        show "(smap f (siterate g (p, q, s)), s) \<in> \<langle>T\<rangle> stream_rel"
+          using 1 2 3 unfolding Q_def g_def by (coinduction arbitrary: p q s) (fastforce)
+        show "A.run (smap f (siterate g (p, q, s))) p"
+          using 1 2 3 unfolding Q_def g_def by (coinduction arbitrary: p q s) (fastforce)
+      qed
+    qed
+    show ?thesis unfolding transition_system.runs_def set_rel_def using 1 2 by force
   qed
 
 end
